libcrux-iot/sha3/proofs/fstar/extraction/Libcrux_iot_sha3.Incremental.Bundle.fst
@@ -1,0 +1,342 @@
+module Libcrux_iot_sha3.Incremental.Bundle
+#set-options "--fuel 0 --ifuel 1 --z3rlimit 15"
+open FStar.Mul
+open Core_models
+
+/// An unbuffered XOF state.
+type t_UnbufferedXofState = { f_state:Libcrux_iot_sha3.State.t_KeccakState }
+
+[@@ FStar.Tactics.Typeclasses.tcinstance]
+assume
+val impl_2': Core_models.Fmt.t_Debug t_UnbufferedXofState
+
+unfold
+let impl_2 = impl_2'
+
+let impl: Core_models.Clone.t_Clone t_UnbufferedXofState =
+  { f_clone = (fun x -> x); f_clone_pre = (fun _ -> True); f_clone_post = (fun _ _ -> True) }
+
+[@@ FStar.Tactics.Typeclasses.tcinstance]
+assume
+val impl_1': Core_models.Marker.t_Copy t_UnbufferedXofState
+
+unfold
+let impl_1 = impl_1'
+
+/// Input-buffering SHAKE128 state
+type t_Shake128Xof = { f_state:Libcrux_iot_sha3.Keccak.t_KeccakXofState (mk_usize 168) }
+
+/// Input-buffering SHAKE256 state
+type t_Shake256Xof = { f_state:Libcrux_iot_sha3.Keccak.t_KeccakXofState (mk_usize 136) }
+
+/// Create a new SHAKE-128 state object.
+let shake128_init (_: Prims.unit) : t_UnbufferedXofState =
+  { f_state = Libcrux_iot_sha3.State.impl_KeccakState__new () } <: t_UnbufferedXofState
+
+/// Absorb
+let shake128_absorb_final (s: t_UnbufferedXofState) (data0: t_Slice u8)
+    : Prims.Pure t_UnbufferedXofState
+      (requires (Core_models.Slice.impl__len #u8 data0 <: usize) <. mk_usize 168)
+      (fun _ -> Prims.l_True) =
+  let s:t_UnbufferedXofState =
+    {
+      s with
+      f_state
+      =
+      Libcrux_iot_sha3.Keccak.absorb_final (mk_usize 168)
+        (mk_u8 31)
+        s.f_state
+        data0
+        (mk_usize 0)
+        (Core_models.Slice.impl__len #u8 data0 <: usize)
+    }
+    <:
+    t_UnbufferedXofState
+  in
+  s
+
+/// Squeeze three blocks
+let shake128_squeeze_first_three_blocks (s: t_UnbufferedXofState) (out0: t_Slice u8)
+    : Prims.Pure (t_UnbufferedXofState & t_Slice u8)
+      (requires
+        (Core_models.Slice.impl__len #u8 out0 <: usize) >=. (mk_usize 3 *! mk_usize 168 <: usize))
+      (fun _ -> Prims.l_True) =
+  let (tmp0: Libcrux_iot_sha3.State.t_KeccakState), (tmp1: t_Slice u8) =
+    Libcrux_iot_sha3.Keccak.squeeze_first_three_blocks (mk_usize 168) s.f_state out0
+  in
+  let s:t_UnbufferedXofState = { s with f_state = tmp0 } <: t_UnbufferedXofState in
+  let out0:t_Slice u8 = tmp1 in
+  let _:Prims.unit = () in
+  s, out0 <: (t_UnbufferedXofState & t_Slice u8)
+
+/// Squeeze five blocks
+let shake128_squeeze_first_five_blocks (s: t_UnbufferedXofState) (out0: t_Slice u8)
+    : Prims.Pure (t_UnbufferedXofState & t_Slice u8)
+      (requires
+        (Core_models.Slice.impl__len #u8 out0 <: usize) >=. (mk_usize 5 *! mk_usize 168 <: usize))
+      (fun _ -> Prims.l_True) =
+  let (tmp0: Libcrux_iot_sha3.State.t_KeccakState), (tmp1: t_Slice u8) =
+    Libcrux_iot_sha3.Keccak.squeeze_first_five_blocks (mk_usize 168) s.f_state out0
+  in
+  let s:t_UnbufferedXofState = { s with f_state = tmp0 } <: t_UnbufferedXofState in
+  let out0:t_Slice u8 = tmp1 in
+  let _:Prims.unit = () in
+  s, out0 <: (t_UnbufferedXofState & t_Slice u8)
+
+/// Squeeze another block
+let shake128_squeeze_next_block (s: t_UnbufferedXofState) (out0: t_Slice u8)
+    : Prims.Pure (t_UnbufferedXofState & t_Slice u8)
+      (requires (Core_models.Slice.impl__len #u8 out0 <: usize) >=. mk_usize 168)
+      (fun _ -> Prims.l_True) =
+  let (tmp0: Libcrux_iot_sha3.State.t_KeccakState), (tmp1: t_Slice u8) =
+    Libcrux_iot_sha3.Keccak.squeeze_next_block (mk_usize 168) s.f_state out0
+  in
+  let s:t_UnbufferedXofState = { s with f_state = tmp0 } <: t_UnbufferedXofState in
+  let out0:t_Slice u8 = tmp1 in
+  let _:Prims.unit = () in
+  s, out0 <: (t_UnbufferedXofState & t_Slice u8)
+
+/// Create a new SHAKE-256 state object.
+let shake256_init (_: Prims.unit) : t_UnbufferedXofState =
+  { f_state = Libcrux_iot_sha3.State.impl_KeccakState__new () } <: t_UnbufferedXofState
+
+/// Absorb some data for SHAKE-256 for the last time
+let shake256_absorb_final (s: t_UnbufferedXofState) (data: t_Slice u8)
+    : Prims.Pure t_UnbufferedXofState
+      (requires (Core_models.Slice.impl__len #u8 data <: usize) <. mk_usize 136)
+      (fun _ -> Prims.l_True) =
+  let s:t_UnbufferedXofState =
+    {
+      s with
+      f_state
+      =
+      Libcrux_iot_sha3.Keccak.absorb_final (mk_usize 136)
+        (mk_u8 31)
+        s.f_state
+        data
+        (mk_usize 0)
+        (Core_models.Slice.impl__len #u8 data <: usize)
+    }
+    <:
+    t_UnbufferedXofState
+  in
+  s
+
+/// Squeeze the first SHAKE-256 block
+let shake256_squeeze_first_block (s: t_UnbufferedXofState) (out: t_Slice u8)
+    : Prims.Pure (t_UnbufferedXofState & t_Slice u8)
+      (requires (Core_models.Slice.impl__len #u8 out <: usize) >=. mk_usize 136)
+      (fun _ -> Prims.l_True) =
+  let out:t_Slice u8 = Libcrux_iot_sha3.Keccak.squeeze_first_block (mk_usize 136) s.f_state out in
+  s, out <: (t_UnbufferedXofState & t_Slice u8)
+
+/// Squeeze the next SHAKE-256 block
+let shake256_squeeze_next_block (s: t_UnbufferedXofState) (out: t_Slice u8)
+    : Prims.Pure (t_UnbufferedXofState & t_Slice u8)
+      (requires (Core_models.Slice.impl__len #u8 out <: usize) >=. mk_usize 136)
+      (fun _ -> Prims.l_True) =
+  let (tmp0: Libcrux_iot_sha3.State.t_KeccakState), (tmp1: t_Slice u8) =
+    Libcrux_iot_sha3.Keccak.squeeze_next_block (mk_usize 136) s.f_state out
+  in
+  let s:t_UnbufferedXofState = { s with f_state = tmp0 } <: t_UnbufferedXofState in
+  let out:t_Slice u8 = tmp1 in
+  let _:Prims.unit = () in
+  s, out <: (t_UnbufferedXofState & t_Slice u8)
+
+class t_Sealed (v_Self: Type0) = { __marker_trait_t_Sealed:Prims.unit }
+
+/// Interface for an input-buffering Extendable Output Function
+/// (XOF)
+class t_Xof (v_Self: Type0) (v_RATE: usize) = {
+  [@@@ FStar.Tactics.Typeclasses.no_method]_super_i0:t_Sealed v_Self;
+  f_new_pre:Prims.unit -> Type0;
+  f_new_post:Prims.unit -> v_Self -> Type0;
+  f_new:x0: Prims.unit -> Prims.Pure v_Self (f_new_pre x0) (fun result -> f_new_post x0 result);
+  f_absorb_pre:v_Self -> t_Slice u8 -> Type0;
+  f_absorb_post:v_Self -> t_Slice u8 -> v_Self -> Type0;
+  f_absorb:x0: v_Self -> x1: t_Slice u8
+    -> Prims.Pure v_Self (f_absorb_pre x0 x1) (fun result -> f_absorb_post x0 x1 result);
+  f_absorb_final_pre:v_Self -> t_Slice u8 -> Type0;
+  f_absorb_final_post:v_Self -> t_Slice u8 -> v_Self -> Type0;
+  f_absorb_final:x0: v_Self -> x1: t_Slice u8
+    -> Prims.Pure v_Self (f_absorb_final_pre x0 x1) (fun result -> f_absorb_final_post x0 x1 result);
+  f_squeeze_pre:v_Self -> t_Slice u8 -> Type0;
+  f_squeeze_post:v_Self -> t_Slice u8 -> (v_Self & t_Slice u8) -> Type0;
+  f_squeeze:x0: v_Self -> x1: t_Slice u8
+    -> Prims.Pure (v_Self & t_Slice u8)
+        (f_squeeze_pre x0 x1)
+        (fun result -> f_squeeze_post x0 x1 result)
+}
+
+[@@ FStar.Tactics.Typeclasses.tcinstance]
+let _ = fun (v_Self:Type0) (v_RATE:usize) {|i: t_Xof v_Self v_RATE|} -> i._super_i0
+
+[@@ FStar.Tactics.Typeclasses.tcinstance]
+let impl__from__private: t_Sealed t_Shake128Xof = { __marker_trait_t_Sealed = () }
+
+[@@ FStar.Tactics.Typeclasses.tcinstance]
+let impl_3: t_Xof t_Shake128Xof (mk_usize 168) =
+  {
+    _super_i0 = FStar.Tactics.Typeclasses.solve;
+    f_new_pre = (fun (_: Prims.unit) -> true);
+    f_new_post = (fun (_: Prims.unit) (out: t_Shake128Xof) -> true);
+    f_new
+    =
+    (fun (_: Prims.unit) ->
+        { f_state = Libcrux_iot_sha3.Keccak.impl__new (mk_usize 168) () } <: t_Shake128Xof);
+    f_absorb_pre
+    =
+    (fun (self_: t_Shake128Xof) (input: t_Slice u8) ->
+        self_.f_state.Libcrux_iot_sha3.Keccak.f_buf_len <. mk_usize 168 &&
+        ((Rust_primitives.Hax.Int.from_machine (Core_models.Slice.impl__len #u8 input <: usize)
+            <:
+            Hax_lib.Int.t_Int) +
+          (Rust_primitives.Hax.Int.from_machine self_.f_state.Libcrux_iot_sha3.Keccak.f_buf_len
+            <:
+            Hax_lib.Int.t_Int)
+          <:
+          Hax_lib.Int.t_Int) <=
+        (Rust_primitives.Hax.Int.from_machine Core_models.Num.impl_usize__MAX <: Hax_lib.Int.t_Int));
+    f_absorb_post = (fun (self: t_Shake128Xof) (input: t_Slice u8) (out: t_Shake128Xof) -> true);
+    f_absorb
+    =
+    (fun (self: t_Shake128Xof) (input: t_Slice u8) ->
+        let self:t_Shake128Xof =
+          {
+            self with
+            f_state = Libcrux_iot_sha3.Keccak.impl__absorb (mk_usize 168) self.f_state input
+          }
+          <:
+          t_Shake128Xof
+        in
+        self);
+    f_absorb_final_pre
+    =
+    (fun (self_: t_Shake128Xof) (input: t_Slice u8) ->
+        self_.f_state.Libcrux_iot_sha3.Keccak.f_buf_len <. mk_usize 168 &&
+        ((Rust_primitives.Hax.Int.from_machine (Core_models.Slice.impl__len #u8 input <: usize)
+            <:
+            Hax_lib.Int.t_Int) +
+          (Rust_primitives.Hax.Int.from_machine self_.f_state.Libcrux_iot_sha3.Keccak.f_buf_len
+            <:
+            Hax_lib.Int.t_Int)
+          <:
+          Hax_lib.Int.t_Int) <=
+        (Rust_primitives.Hax.Int.from_machine Core_models.Num.impl_usize__MAX <: Hax_lib.Int.t_Int));
+    f_absorb_final_post
+    =
+    (fun (self: t_Shake128Xof) (input: t_Slice u8) (out: t_Shake128Xof) -> true);
+    f_absorb_final
+    =
+    (fun (self: t_Shake128Xof) (input: t_Slice u8) ->
+        let self:t_Shake128Xof =
+          {
+            self with
+            f_state
+            =
+            Libcrux_iot_sha3.Keccak.impl__absorb_final (mk_usize 168) (mk_u8 31) self.f_state input
+          }
+          <:
+          t_Shake128Xof
+        in
+        self);
+    f_squeeze_pre = (fun (self: t_Shake128Xof) (out: t_Slice u8) -> true);
+    f_squeeze_post
+    =
+    (fun (self: t_Shake128Xof) (out: t_Slice u8) (out1: (t_Shake128Xof & t_Slice u8)) -> true);
+    f_squeeze
+    =
+    fun (self: t_Shake128Xof) (out: t_Slice u8) ->
+      let (tmp0: Libcrux_iot_sha3.Keccak.t_KeccakXofState (mk_usize 168)), (tmp1: t_Slice u8) =
+        Libcrux_iot_sha3.Keccak.impl__squeeze (mk_usize 168) self.f_state out
+      in
+      let self:t_Shake128Xof = { self with f_state = tmp0 } <: t_Shake128Xof in
+      let out:t_Slice u8 = tmp1 in
+      let _:Prims.unit = () in
+      self, out <: (t_Shake128Xof & t_Slice u8)
+  }
+
+[@@ FStar.Tactics.Typeclasses.tcinstance]
+let impl_1__from__private: t_Sealed t_Shake256Xof = { __marker_trait_t_Sealed = () }
+
+[@@ FStar.Tactics.Typeclasses.tcinstance]
+let impl_4: t_Xof t_Shake256Xof (mk_usize 136) =
+  {
+    _super_i0 = FStar.Tactics.Typeclasses.solve;
+    f_new_pre = (fun (_: Prims.unit) -> true);
+    f_new_post = (fun (_: Prims.unit) (out: t_Shake256Xof) -> true);
+    f_new
+    =
+    (fun (_: Prims.unit) ->
+        { f_state = Libcrux_iot_sha3.Keccak.impl__new (mk_usize 136) () } <: t_Shake256Xof);
+    f_absorb_pre
+    =
+    (fun (self_: t_Shake256Xof) (input: t_Slice u8) ->
+        self_.f_state.Libcrux_iot_sha3.Keccak.f_buf_len <. mk_usize 136 &&
+        ((Rust_primitives.Hax.Int.from_machine (Core_models.Slice.impl__len #u8 input <: usize)
+            <:
+            Hax_lib.Int.t_Int) +
+          (Rust_primitives.Hax.Int.from_machine self_.f_state.Libcrux_iot_sha3.Keccak.f_buf_len
+            <:
+            Hax_lib.Int.t_Int)
+          <:
+          Hax_lib.Int.t_Int) <=
+        (Rust_primitives.Hax.Int.from_machine Core_models.Num.impl_usize__MAX <: Hax_lib.Int.t_Int));
+    f_absorb_post = (fun (self: t_Shake256Xof) (input: t_Slice u8) (out: t_Shake256Xof) -> true);
+    f_absorb
+    =
+    (fun (self: t_Shake256Xof) (input: t_Slice u8) ->
+        let self:t_Shake256Xof =
+          {
+            self with
+            f_state = Libcrux_iot_sha3.Keccak.impl__absorb (mk_usize 136) self.f_state input
+          }
+          <:
+          t_Shake256Xof
+        in
+        self);
+    f_absorb_final_pre
+    =
+    (fun (self_: t_Shake256Xof) (input: t_Slice u8) ->
+        self_.f_state.Libcrux_iot_sha3.Keccak.f_buf_len <. mk_usize 136 &&
+        ((Rust_primitives.Hax.Int.from_machine (Core_models.Slice.impl__len #u8 input <: usize)
+            <:
+            Hax_lib.Int.t_Int) +
+          (Rust_primitives.Hax.Int.from_machine self_.f_state.Libcrux_iot_sha3.Keccak.f_buf_len
+            <:
+            Hax_lib.Int.t_Int)
+          <:
+          Hax_lib.Int.t_Int) <=
+        (Rust_primitives.Hax.Int.from_machine Core_models.Num.impl_usize__MAX <: Hax_lib.Int.t_Int));
+    f_absorb_final_post
+    =
+    (fun (self: t_Shake256Xof) (input: t_Slice u8) (out: t_Shake256Xof) -> true);
+    f_absorb_final
+    =
+    (fun (self: t_Shake256Xof) (input: t_Slice u8) ->
+        let self:t_Shake256Xof =
+          {
+            self with
+            f_state
+            =
+            Libcrux_iot_sha3.Keccak.impl__absorb_final (mk_usize 136) (mk_u8 31) self.f_state input
+          }
+          <:
+          t_Shake256Xof
+        in
+        self);
+    f_squeeze_pre = (fun (self: t_Shake256Xof) (out: t_Slice u8) -> true);
+    f_squeeze_post
+    =
+    (fun (self: t_Shake256Xof) (out: t_Slice u8) (out1: (t_Shake256Xof & t_Slice u8)) -> true);
+    f_squeeze
+    =
+    fun (self: t_Shake256Xof) (out: t_Slice u8) ->
+      let (tmp0: Libcrux_iot_sha3.Keccak.t_KeccakXofState (mk_usize 136)), (tmp1: t_Slice u8) =
+        Libcrux_iot_sha3.Keccak.impl__squeeze (mk_usize 136) self.f_state out
+      in
+      let self:t_Shake256Xof = { self with f_state = tmp0 } <: t_Shake256Xof in
+      let out:t_Slice u8 = tmp1 in
+      let _:Prims.unit = () in
+      self, out <: (t_Shake256Xof & t_Slice u8)
+  }
