libcrux-iot/sha3/proofs/fstar/extraction/Libcrux_iot_sha3.Incremental.Private.fst
@@ -1,0 +1,10 @@
+module Libcrux_iot_sha3.Incremental.Private
+#set-options "--fuel 0 --ifuel 1 --z3rlimit 15"
+open FStar.Mul
+open Core_models
+
+include Libcrux_iot_sha3.Incremental.Bundle {t_Sealed as t_Sealed}
+
+include Libcrux_iot_sha3.Incremental.Bundle {impl__from__private as impl}
+
+include Libcrux_iot_sha3.Incremental.Bundle {impl_1__from__private as impl_1}
